Prefix(:=<http://daml.umbc.edu/ontologies/cobra/0.4/calendarclock#>)
Prefix(owl:=<http://www.w3.org/2002/07/owl#>)
Prefix(rdf:=<http://www.w3.org/1999/02/22-rdf-syntax-ns#>)
Prefix(xml:=<http://www.w3.org/XML/1998/namespace>)
Prefix(xsd:=<http://www.w3.org/2001/XMLSchema#>)
Prefix(rdfs:=<http://www.w3.org/2000/01/rdf-schema#>)


Ontology(<http://daml.umbc.edu/ontologies/cobra/0.4/calendarclock>
Annotation(rdfs:label "COBRA-ONT Calendar/Clock Ontology")
Annotation(owl:versionInfo "0.4")
Annotation(rdfs:comment "
      An ontology for describing calendar and clock time. 

      Parts of this ontology are adopted from the time-entry ontology
      developed by Feng Pan and Jerry R. Hobbs (USC/ISI) and DAML-Time.
    ")

Declaration(Class(:CalendarDescription))
AnnotationAssertion(rdfs:label :CalendarDescription "CalendarDescription")
AnnotationAssertion(<http://attempto.ifi.uzh.ch/ace_lexicon#CN_pl> :CalendarDescription "CalendarDescriptions")
AnnotationAssertion(<http://attempto.ifi.uzh.ch/ace_lexicon#CN_sg> :CalendarDescription "CalendarDescription")
SubClassOf(:CalendarDescription DataMaxCardinality(1 :dateOfMonth))
SubClassOf(:CalendarDescription DataMaxCardinality(1 :month))
SubClassOf(:CalendarDescription DataMaxCardinality(1 :year))
Declaration(Class(:ClockDescription))
AnnotationAssertion(<http://attempto.ifi.uzh.ch/ace_lexicon#CN_sg> :ClockDescription "ClockDescription")
AnnotationAssertion(rdfs:label :ClockDescription "ClockDescription")
AnnotationAssertion(<http://attempto.ifi.uzh.ch/ace_lexicon#CN_pl> :ClockDescription "ClockDescriptions")
SubClassOf(:ClockDescription DataMaxCardinality(1 :hourOfDay))
SubClassOf(:ClockDescription DataMaxCardinality(1 :minute))
SubClassOf(:ClockDescription DataMaxCardinality(1 :second))
Declaration(DataProperty(:dateOfMonth))
AnnotationAssertion(rdfs:label :dateOfMonth "dateOfMonth")
AnnotationAssertion(<http://attempto.ifi.uzh.ch/ace_lexicon#TV_sg> :dateOfMonth "dateOfMonths")
AnnotationAssertion(<http://attempto.ifi.uzh.ch/ace_lexicon#TV_pl> :dateOfMonth "dateOfMonth")
AnnotationAssertion(<http://attempto.ifi.uzh.ch/ace_lexicon#TV_vbg> :dateOfMonth "dateOfMonthed")
DataPropertyRange(:dateOfMonth xsd:gDay)
Declaration(DataProperty(:hourOfDay))
AnnotationAssertion(rdfs:comment :hourOfDay "
      A non-negative integer that represents the hour of the day in
      the 24-hour clock (e.g., at 10:04:32 PM, the hourOfDay is 10)
    ")
AnnotationAssertion(<http://attempto.ifi.uzh.ch/ace_lexicon#TV_pl> :hourOfDay "hourOfDay")
AnnotationAssertion(rdfs:label :hourOfDay "hourOfDay")
AnnotationAssertion(<http://attempto.ifi.uzh.ch/ace_lexicon#TV_sg> :hourOfDay "hourOfDays")
AnnotationAssertion(<http://attempto.ifi.uzh.ch/ace_lexicon#TV_vbg> :hourOfDay "hourOfDayed")
DataPropertyRange(:hourOfDay xsd:nonNegativeInteger)
Declaration(DataProperty(:minute))
AnnotationAssertion(<http://attempto.ifi.uzh.ch/ace_lexicon#TV_pl> :minute "minute")
AnnotationAssertion(rdfs:label :minute "minute")
AnnotationAssertion(<http://attempto.ifi.uzh.ch/ace_lexicon#TV_sg> :minute "minutes")
AnnotationAssertion(<http://attempto.ifi.uzh.ch/ace_lexicon#TV_vbg> :minute "minuted")
AnnotationAssertion(rdfs:comment :minute "
      A non-negative integer that represents the minute within the
      hour (e.g., at 10:02:23 PM, the minute is 2).
    ")
DataPropertyRange(:minute xsd:nonNegativeInteger)
Declaration(DataProperty(:month))
AnnotationAssertion(<http://attempto.ifi.uzh.ch/ace_lexicon#TV_sg> :month "months")
AnnotationAssertion(rdfs:label :month "month")
AnnotationAssertion(<http://attempto.ifi.uzh.ch/ace_lexicon#TV_vbg> :month "monthed")
AnnotationAssertion(<http://attempto.ifi.uzh.ch/ace_lexicon#TV_pl> :month "month")
DataPropertyRange(:month xsd:gMonth)
Declaration(DataProperty(:second))
AnnotationAssertion(<http://attempto.ifi.uzh.ch/ace_lexicon#TV_vbg> :second "seconded")
AnnotationAssertion(rdfs:comment :second "
      A non-negative integer that represents the second within the
      minute (e.g., at 10:02:23 PM, the minute is 23).
    ")
AnnotationAssertion(rdfs:label :second "second")
AnnotationAssertion(<http://attempto.ifi.uzh.ch/ace_lexicon#TV_sg> :second "seconds")
AnnotationAssertion(<http://attempto.ifi.uzh.ch/ace_lexicon#TV_pl> :second "second")
DataPropertyRange(:second xsd:nonNegativeInteger)
Declaration(DataProperty(:year))
AnnotationAssertion(rdfs:label :year "year")
AnnotationAssertion(<http://attempto.ifi.uzh.ch/ace_lexicon#TV_sg> :year "years")
AnnotationAssertion(<http://attempto.ifi.uzh.ch/ace_lexicon#TV_vbg> :year "yeared")
AnnotationAssertion(<http://attempto.ifi.uzh.ch/ace_lexicon#TV_pl> :year "year")
DataPropertyRange(:year xsd:gYear)
)
